\documentclass{article}
\usepackage[utf8]{inputenc}
\usepackage{amsmath}

\title{Assignment 2}
\author{Swapnil Sirsat }
\date{January 2021}

\begin{document}

\maketitle

\section*{Question 1}
If $A$ = \begin{pmatrix} 3 & \sqrt{3} & 2 \\ 4 & 2 & 0 \\ \end{pmatrix} and $B$ = \begin{pmatrix} 2 & -1 & 2 \\ 1 & 2 & 4 \\ \end{pmatrix} verify that \\
$(i) (A')' = A$ \\
$(ii)(A + B)' = A' + B'$ \\
$(iii) (kB)' = kB'$ ,where k is any constant. \\
\section*{Solution :}
\subsection*{$(i)$ $(A')' = A$ } 
Given $A$ = \begin{pmatrix} 3 & \sqrt{3} & 2 \\ 4 & 2 & 0 \\ \end{pmatrix} \\
Thus, \\
$A'$ = \begin{pmatrix}  3 & 4 \\ \sqrt{3} & 2 \\ 2 & 0 \\ \end{pmatrix} \\
Now, \\ 
$(A')'$ =  $\begin{pmatrix}  3 & 4 \\ \sqrt{3} & 2 \\ 2 & 0 \\ \end{pmatrix}'$  = \begin{pmatrix} 3 & \sqrt{3} & 2 \\ 4 & 2 & 0 \\ \end{pmatrix} = $A$ \\
Hence, $(A')$' = $A$
\subsection*{$(ii)$ $(A + B)' = A' + B'$}
$A$ =  \begin{pmatrix} 3 & \sqrt{3} & 2 \\ 4 & 2 & 0 \\ \end{pmatrix} and $B$ = \begin{pmatrix} 2 & -1 & 2 \\ 1 & 2 & 4 \\ \end{pmatrix} \\
$A+B$ = \begin{pmatrix} 3 & \sqrt{3} & 2 \\ 4 & 2 & 0 \\ \end{pmatrix}  $+$ \begin{pmatrix} 2 & -1 & 2 \\ 1 & 2 & 4 \\ \end{pmatrix} = \begin{pmatrix} 5 & \sqrt{3}-1 & 4 \\ 5 & 4 & 4  \end{pmatrix} \\
$(A+B)'$ =  \begin{pmatrix} 5 & 5 \\ \sqrt{3}-1 & 4 \\ 4 & 4 \\ \end{pmatrix} \\ 
Now, \\
$A'$ = \begin{pmatrix}  3 & 4 \\ \sqrt{3} & 2 \\ 2 & 0 \\ \end{pmatrix} and $B'$ = \begin{pmatrix} 2 & 1 \\ -1 & 2 \\ 2 & 4  \end{pmatrix} \\ 
$A' + B'$ = \begin{pmatrix} 5 & 5 \\ \sqrt{3}-1 & 4 \\ 4 & 4 \\ \end{pmatrix} = $(A+B)'$\\
therefore, $A' + B'$ = $(A+B)'$
\subsection*{$(iii)$ $(kB)' = kB'$}
$B$ = \begin{pmatrix} 2 & -1 & 2 \\ 1 & 2 & 4 \\ \end{pmatrix} \\
$kB$ = \begin{pmatrix} 2k & -1k & 2k \\ 1k & 2k & 4k \\ \end{pmatrix} \\
$(kB)'$ = \begin{pmatrix} 2k & 1k \\ -1k & 2k \\ 2k & 4k \end{pmatrix} \\
now, $B'$ = \begin{pmatrix} 2 & 1 \\ -1 & 2 \\ 2 & 4  \end{pmatrix} \\
$kB'$ =  \begin{pmatrix} 2k & 1k \\ -1k & 2k \\ 2k & 4k  \end{pmatrix} = $(kB)'$ \\
therefore, $kB'$ = $(kB)'$ 
\newpage

\section*{Question 2}
If $A$ = \begin{pmatrix} 2 \\ 4 \\ 5 \end{pmatrix}, $B$ = \begin{pmatrix} 1 & 3 & -6 \end{pmatrix}, verify that $(AB)' = B'A'$

\section*{Solution :}
$A$ = \begin{pmatrix} 2 \\ 4 \\ 5 \end{pmatrix} and $B$ = \begin{pmatrix} 1 & 3 & -6 \end{pmatrix}\\
$A'$ = \begin{pmatrix}  2 & 4 & 5 \end{pmatrix} and $B'$ = \begin{pmatrix} 1 \\ 3 \\ -6 \end{pmatrix}\\
now, \\
$AB$ = \begin{pmatrix} 2 \\ 4 \\ 5 \end{pmatrix}\begin{pmatrix} 1 & 3 & -6 \end{pmatrix} \\
$AB$ = \begin{pmatrix} 2 & 6 & -12 \\ 4 & 12 & -24 \\ 5 & 15 & -30 \\  \end{pmatrix} \\
$(AB)'$ = \begin{pmatrix} 2 & 4 & 5 \\ 6 & 12 & 15 \\ -12 & -24 & -30 \end{pmatrix} \\

Now,\\
$B'A'$ = \begin{pmatrix} 1 \\ 3 \\ -6 \end{pmatrix}\begin{pmatrix}  2 & 4 & 5 \end{pmatrix} \\
$B'A'$ = \begin{pmatrix} 2 & 4 & 5 \\ 6 & 12 & 15 \\ -12 & -24 & -30\\\end{pmatrix} = $(AB)'$ \\
therefore, $B'A'$ = $(AB)'$




\end{document}
